document pattern aliases

Pattern_Aliases.thy
@@ -1,6 +1,33 @@
+(*  Title:      HOL/Library/Pattern_Aliases.thy
+    Author:     Lars Hupel, Ondrej Kuncar
+*)
+
+section \<open>Input syntax for pattern aliases (or ``as-patterns'' in Haskell)\<close>
+
 theory Pattern_Aliases
 imports Main
 begin
+
+text \<open>
+  Most functional languages (Haskell, ML, Scala) support aliases in patterns. This allows to refer
+  to a subpattern with a variable name. This theory implements this using a check phase. It works
+  well for function definitions (see usage below).
+
+  The following caveats should be kept in mind:
+  \<^item> The translation expects a term of the form @{prop "f x y = rhs"}, where \<open>x\<close> and \<open>y\<close> are patterns
+    that may contain aliases. The result of the translation is a nested @{const Let}-expression on
+    the right hand side. The code generator \<^emph>\<open>does not\<close> print Isabelle pattern aliases to target
+    language pattern aliases.
+  \<^item> The translation does not process nested equalities; only the top-level equality is translated.
+  \<^item> Terms that do not adhere to the above shape may either stay untranslated or produce an error
+    message. The @{command fun} command will complain if pattern aliases are left untranslated.
+    In particular, there are no checks whether the patterns are wellformed or linear.
+  \<^item> There is no corresonding uncheck phase, because it is unclear in which situations the
+    translation should be reversed.
+\<close>
+
+
+subsection \<open>Definition\<close>
 
 consts as :: "'a \<Rightarrow> 'a \<Rightarrow> 'a"
 
@@ -19,17 +46,14 @@ fun all_Frees t =
 
 in
 
-(* doesn't check that defined constant doesn't occur to the left of =: *)
-(* doesn't check linearity *)
-
 fun check_pattern_syntax t =
   case strip_all t of
     (vars, @{const Trueprop} $ (Const (@{const_name HOL.eq}, _) $ lhs $ rhs)) =>
       let
-        fun go (Const (@{const_name as}, _) $ var $ pat, rhs) =
+        fun go (Const (@{const_name as}, _) $ pat $ var, rhs) =
               let
                 val (pat', rhs') = go (pat, rhs)
-                val _ = if is_Free var then () else error "no can do"
+                val _ = if is_Free var then () else error "Left-hand side of =: must be a free variable"
                 val rhs'' =
                   Const (@{const_name Let}, let_typ (fastype_of var) (fastype_of rhs)) $
                     pat' $ lambda var rhs'
@@ -54,9 +78,9 @@ fun check_pattern_syntax t =
 end
 \<close>
 
-bundle pattern_syntax begin
+bundle pattern_aliases begin
 
-  notation as (infixr "=:" 65)
+  notation as (infixr "=:" 1)
 
   declaration \<open>K (Syntax_Phases.term_check 98 "pattern_syntax" (K (map check_pattern_syntax)))\<close>
 
@@ -64,15 +88,26 @@ end
 
 hide_const (open) as
 
-context includes pattern_syntax begin
 
-term "\<And>x y ys. bla (x =: (y # ys)) = x @ x"
+subsection \<open>Usage\<close>
 
-fun bla where
-"bla [] = []" |
-"bla (x =: (y # (x' =: (y' # ys)))) = x @ x'"
+context includes pattern_aliases begin
 
-thm bla.simps[unfolded Let_def]
+text \<open>Not very useful for plain definitions, but works anyway.\<close>
+
+private definition "test_1 x (y =: z) = y + z"
+
+lemma "test_1 x y = y + y"
+by (rule test_1_def[unfolded Let_def])
+
+text \<open>Very useful for function definitions.\<close>
+
+private fun test_2 where
+"test_2 (y # (y' # ys =: x') =: x) = x @ x'" |
+"test_2 _ = []"
+
+lemma "test_2 (y # y' # ys) = (y # y' # ys) @ y' # ys"
+by (rule test_2.simps[unfolded Let_def])
 
 end
 
